src/MicroSail/Syntax.v
@@ -96,6 +96,7 @@ Module Type TermKit.
   (* Names of registers. *)
   Parameter Inline 𝑹𝑬𝑮 : Ty -> Set.
   Declare Instance 𝑹𝑬𝑮_eq_dec : EqDec (sigT 𝑹𝑬𝑮).
+  Declare Instance 𝑹𝑬𝑮_finite : finite.Finite (sigT 𝑹𝑬𝑮).
 
 End TermKit.
 
